\section{Operatorial representation}

\begin{definition}[\textit{Backward shift operator}]
    The backward shift operator $z^{-1}$ is defined as: 
    \[z^{-1}\cdot x(t)=x(t-1)\]
\end{definition}
\begin{definition}[\textit{Forward shift operator}]
    The forward shift operator $z$ is defined as: 
    \[z\cdot x(t)=x(t+1)\]
\end{definition}
The properties of the backward and forward shift operators are:
\begin{enumerate}
    \item Linearity:
        \[z^{-1}\left(ax(t)+by(t) \right)=ax(t-1)+by(t-1)\]
    \item Recursive application: 
        \[z^{-1}\left(z^{-1}\left(z^{-1}\left(x(t)\right)\right)\right)=z^{-1}\left(z^{-1}\left(x(t-1)\right)\right)=z^{-1}\left(x(t-2)\right)=x(t-3)=z^{-3}x(t)\]
    \item Linear composition: 
        \[\left(az^{-1}+bz+cz^{-3}+dz^2\right)=ax(t-1)+bx(t+1)+cx(t-3)+dx(t+2)\]
\end{enumerate} 