\section{Processes with non-zero mean}

Consider an ARMA($m,n$) process:
\[y(t)=a_1y(t-1)+a_2y(t-2)+\dots+a_my(t-m)+c_0e(t)+c_1e(t-1)+\dots+c_ne(t-n) \]
Here, $e(t)\sim WN(\mu,\lambda^2)$.
In operatorial representation, this process can be expressed as:
\[y(t)=\dfrac{c_0+c_1z^{-1}+\dots+c_nz^{-n}}{1- a_1z^{-1}-a_2z^{-2}-\dots-a_mz^{-m}}e(t)=\dfrac{C(z)}{A(z)}e(t)\]

\paragraph*{Mean value}
The mean is computed as:
\begin{align*}
    m_y=    &= \mathbb{E}\left[y(t)\right]  \\
            &= \mathbb{E}\left[a_1y(t-1)+\dots+a_my(t-m)+c_0e(t)+\dots+c_ne(t-n)\right] \\
            &= a_1\mathbb{E}\left[y(t-1)\right]+\dots+a_m\mathbb{E}\left[y(t-m)\right]+c_0\underbrace{\mathbb{E}\left[e(t)\right]}_{m_e} +\dots+c_n\underbrace{\mathbb{E}\left[e(t-n)\right]}_{m_e} \\
            &= a_1\mathbb{E}\left[y(t-1)\right]+\dots+a_m\mathbb{E}\left[y(t-m)\right]+\left(c_0 +\dots+c_n\right)m_e 
\end{align*}
Assuming that $a_1,a_2,\dots,a_m$ are chosen such that $y(t)$ is a stationary stochastic process with constant mean value, we can rewrite the previous formulation as:
\[m_y=\left(a_1+a_2+\dots+a_m\right)m_y+\left(c_0 +c_1 +\dots+c_n\right)m_e \rightarrow m_y =\dfrac{c_0 +c_1 +\dots+c_n}{1-a_1-a_2-\dots-a_m}m_e\]
Note that the transfer function is computed at $z=1$ (the DC gain of $W(z)$), so we have:
\[m_y=W(1)m_e\]

\paragraph*{Covariance function}
The covariance with a generic $\tau$ is computed as:
\[\gamma_y(\tau)  = \mathbb{E}\left[\left(y(t)-m_y\right)\left(y(t-\tau)-m_y\right)\right]\]
In this case, where $m_y \neq 0$, we have:
\[\mathbb{E}\left[e(t)^2\right]=\mathbb{E}\left[\left(e(t)-\mu\right)^2\right]= \lambda^2\]
and 
\[\mathbb{E}\left[e(t)e(t-1)\right]=\mathbb{E}\left[\left(e(t)-\mu\right)\left(e(t-1)-\mu\right)\right]= 0\]

Therefore,
\begin{align*}
    \lambda^2   &=\mathbb{E}\left[ \left( e(t)-\mu \right)^2 \right] \\
                &=\mathbb{E}\left[ e(t)^2\right] +\mathbb{E}\left[\mu^2\right]-\mathbb{E}\left[2\mu e(t)  \right] \\
                &=\mathbb{E}\left[ e(t)^2\right] +\mu^2-2\mu \mathbb{E}\left[e(t)  \right] \\   
                &=\mathbb{E}\left[ e(t)^2\right] +\mu^2-2\mu^2
\end{align*}
Hence,: 
\[\mathbb{E}\left[e(t)^2\right]=\lambda^2+\mu^2\]

Similarly, we have:
\[0=\mathbb{E}\left[\left(e(t)-\mu\right)\left(e(t-1)-\mu\right)\right] =\mathbb{E}\left[e(t)e(t-1)\right] -\mu^2\]
Therefore,
\[\mathbb{E}\left[e(t)e(t-1)\right]=\mu^2\]

\subsection{Simplification}
To simplify the computation, we define two new unbiased processes:
\[\begin{cases}
    \tilde{y}(t)=y(t)-m_y \\ 
    \tilde{e}(t)=e(t)-m_e
\end{cases}\]
In this case, the expected values become:
\[\begin{cases}
    \mathbb{E}\left[\tilde{y}(t)\right]=\mathbb{E}\left[y(t)-m_y\right]=m_y-m_y=0 \\ 
    \mathbb{E}\left[\tilde{e}(t)\right]=\mathbb{E}\left[e(t)-m_e\right]=m_e-m_e=0
\end{cases}\]

\begin{proof}
    We aim to demonstrate the equivalence between the two processes:
    \begin{align*}
        \tilde{y}(t)    &= y(t)-m_y \\
                        &= a_1y(t-1)+\dots+a_my(t-m)+c_0e(t)+\dots+c_ne(t-n) - m_y \\ 
                        &= a_1\left(\tilde{y}(t-1)+m_y\right)+\dots+a_m\left(\tilde{y}(t-m)+m_y\right)+c_0\left(\tilde{e}(t)+m_e\right)+\dots - m_y \\ 
                        &= a_1\tilde{y}(t-1) +\dots +c_0\tilde{e}(t)+\dots -\left(1 - a_1-\dots-a_m\right)m_y+\left(c_0+\dots+c_n\right)m_e   
    \end{align*}
    However, we know that:
    \[m_y =\dfrac{c_0 +c_1 +\dots+c_n}{1-a_1-a_2-\dots-a_m}m_e\]
    By substitution, we find:
    \begin{align*}
        \tilde{y}(t)    &= a_1\tilde{y}(t-1)  +\dots +c_0\tilde{e}(t)+\dots -\left(1 - a_1-\dots-a_m\right)m_y+\left(c_0+\dots+c_n\right)m_e \\ 
                        &= a_1\tilde{y}(t-1)  +\dots +c_0\tilde{e}(t)+\dots -\left(c_0 +\dots+c_n\right)m_e+\left(c_0+\dots+c_n\right)m_e \\ 
                        &= a_1\tilde{y}(t-1)  +\dots +c_0\tilde{e}(t)+\dots     
    \end{align*}
    Thus, we have shown that the two processes are equivalent.
\end{proof}
Ultimately, we arrive at:
\[ \tilde{y}(t)=a_1\tilde{y}(t-1) +\dots + a_m\tilde{y}(t-m)  +c_0\tilde{e}(t)+c_n\tilde{e}(t-n)+\dots  \qquad \tilde{e}\sim WN(0,\lambda^2)\]
Subsequently, we can compute the covariance as follows:
\[\gamma_{\tilde{y}}(\tau)=\mathbb{E}\left[ \tilde{y}(t)\tilde{y}(t-\tau) \right]=\mathbb{E}\left[ \left(y(t)-m_y\right)\left(y(t-\tau)-m_y\right) \right] =\gamma_y(\tau)\]