\section{Exercise one}

Consider the AR($1$) process: 
\[y(t)=\dfrac{1}{3}y(t-1)+e(t)+2 \qquad e(t)\sim WN(1,1)\]
\begin{enumerate}
    \item Find the transfer function of the system, and verify that it is a stationary stochastic process. 
    \item Compute the expected value. 
    \item Compute the covariance. 
\end{enumerate}

\subsection{Solution}
\begin{enumerate}
    \item We apply the input delay operator, obtaining: 
        \[y(t)=\dfrac{1}{3}z^{-1}y(t)+e(t)+2\]
        By rearranging the terms we have: 
        \[y(t)=\left[\dfrac{z}{z-\frac{1}{3}}\right]\left(e(t)-2\right)\]
        The input is a stationary stochastic process, the poles of the transfer function are: 
        \[z-\frac{1}{3}=0\rightarrow z=\frac{1}{3}\]
        The pole is inside the unity circle, and so this is a stationary stochastic process. 
    \item The expected value is: 
        \[\mathbb{E}\left[y(t)\right]=\mathbb{E}\left[\dfrac{1}{3}y(t-1)+e(t)+2\right]=\dfrac{1}{3}\mathbb{E}\left[y(t-1)\right]+1+2\]
        But we have a stationary stochastic process, so the mean is constant: 
        \[m_y=\dfrac{1}{3}m_y+3\rightarrow m_y=\dfrac{9}{2}\]
    \item We define the unbiased process: 
        \[\begin{cases}
            \tilde{y}(t)=y(t)-m_y \\
            \tilde{e}(t)=e(t)-m_e
        \end{cases}\]
        In our case we have: 
        \[\tilde{y}(t)+\dfrac{9}{2}=\dfrac{1}{3}\left(\tilde{y}(t-1)+\dfrac{9}{2}\right)+\tilde{e}(t)+1+2\rightarrow\tilde{y}(t)=\dfrac{1}{3}\tilde{y}(t-1)+\tilde{e}(t)\]

        We can finally compute the covariance function as: 
        \[\gamma_y(\tau)=\mathbb{E}\left[\tilde{y}(t)\tilde{y}(t-\tau)\right]\]

        We start by the covariance in $\tau=0$: 
        \[\gamma_{\tilde{y}}(0)=\mathbb{E}\left[\tilde{y}(t)^2\right]=\mathbb{E}\left[ \left(\dfrac{1}{3}\tilde{y}(t-1)+\tilde{e}(t)\right)^2\right]=\dfrac{1}{9}\gamma_{\tilde{y}}(0) + 1\rightarrow \gamma_{\tilde{y}}(0)=\dfrac{9}{8}\]
        
        We now compute the covariance in $\tau=1$: 
        \[\gamma_{\tilde{y}}(1)=\mathbb{E}\left[ \tilde{y}(t)\tilde{y}(t-1)\right]=\mathbb{E}\left[ \left(\dfrac{1}{3}\tilde{y}(t-1)+\tilde{e}(t)\right)\tilde{y}(t-1)\right]=\dfrac{1}{3}\gamma_{\tilde{y}}(0)\rightarrow \gamma_{\tilde{y}}(1)=\dfrac{3}{8}\]

        For a generic $\tau$ we have: 
        \[\gamma_{\tilde{y}}(\tau)=\dfrac{1}{3}\gamma_{\tilde{y}}(\tau-1) \qquad \left\lvert \tau \right\rvert \geq 1\]
\end{enumerate}