\section{Exercise one}

Consider an MA(2) process defined by the function:
\[y(t)=e(t)+\dfrac{1}{2}e(t-1)-e(t-2) \qquad e(t)\sim WN(0,1)\]
\begin{enumerate}
    \item Find the transfer function for this system.
    \item Calculate the expected value of the process $y(t)$. 
    \item Compute the covariance function of the process $y(t)$. 
\end{enumerate}

\subsection*{Solution}
\begin{enumerate}
    \item Utilizing the Z-transform, we express the MA(2) process as:
        \[y(t)=e(t)+\dfrac{1}{2}e(t)z^{-1}-e(t)z^{-2}\]
        Grouping the $e(t)$ factor, we obtain:
        \[y(t)=e(t)\left(1+\dfrac{1}{2}z^{-1}-z^{-2}\right)\]
        This yields the polynomial:
        \[W(z)=1+\dfrac{1}{2}z^{-1}-z^{-2}\]
        In normal form, $W(z)$ becomes:
        \[W(z)=\dfrac{z^2+\dfrac{1}{2}z-1}{z^2}\]
    \item The expected value is computed as follows:
        \begin{align*}
            \mathbb{E}\left[y(t)\right]     &= \mathbb{E}\left[e(t)+\dfrac{1}{2}e(t-1)-e(t-2)\right] \\
                                            &= \mathbb{E}\left[e(t)\right]+\mathbb{E}\left[\dfrac{1}{2}e(t-1)\right]-\mathbb{E}\left[e(t-2)\right] \\
                                            &= \underbrace{\mathbb{E}\left[e(t)\right]}_0 +\dfrac{1}{2}\underbrace{\mathbb{E}\left[e(t-1)\right]}_0 -\underbrace{\mathbb{E}\left[e(t-2)\right]}_0  \\
                                            &= 0
        \end{align*}
    \item For the covariance:
        \begin{align*}
            \gamma_y(0)     &= \mathbb{E}\left[{y(t)}^2\right] \\
                            &= \mathbb{E}\left[{\left( e(t)+\dfrac{1}{2}e(t-1)-e(t-2) \right)}^2\right] \\
                            &= \mathbb{E}\left[ {e(t)}^2 + \dfrac{1}{2}{e(t-1)}^2 + {e(t-2)}^2  + \text{cross products} \right] \\
                            &= \underbrace{\mathbb{E}\left[ {e(t)}^2 \right]}_1  + \dfrac{1}{4}\underbrace{\mathbb{E}\left[{e(t-1)}^2\right]}_1  + \underbrace{\mathbb{E}\left[{e(t-2)}^2\right]}_1  + \underbrace{\mathbb{E}\left[\text{cross products}\right]}_0  \\
                            &= 1  + \dfrac{1}{4} + 1\\
                            &= \dfrac{9}{4}
        \end{align*}
        The covariance at lag one is:
        \[\gamma_y(1)=0\]
        We need to compute another time lag since we have two correlated time instants in the formula (square of the same time instant).
        The covariance of two is as follows:
        \[\gamma_y(2)=-1\]
        There is another correlation of the time instant $t-2$, but it is the only one, so for time instants after two, we have a null covariance.
        The final result is:
        \[\begin{cases}
            \gamma_y(0)=\frac{9}{4} \\
            \gamma_y(1)=0 \\
            \gamma_y(2)=-1 \\
            \gamma_y(\tau)=0 \qquad \forall\left\lvert \tau\right\rvert \geq 3
        \end{cases}\]
\end{enumerate}