\section{Exercise two}

Consider the given process:
\[\dfrac{1}{2}y(t)=-\dfrac{1}{3}y(t-1)-\dfrac{1}{18}y(t-2)+3e(t-2)-8e(t-3)-3e(t-4)\]
Here, $e(t)\sim WN(0,1)$. 
Let's compute the one-step ahead predictor.

\subsection*{Solution}
The transfer function is:
\[y(t)=\dfrac{3z^{-2}-8z^{-3}-3z^{-4}}{\frac{1}{2}+\frac{1}{3}z^{-1}+\frac{1}{18}z^{-2}}e(t)\]
We need to rewrite this function in canonical form:
\[y(t)=\dfrac{z^{2}-\frac{8}{3}z-1}{z^2+\frac{2}{3}z+\frac{1}{9}}\frac{3}{\frac{1}{2}}e(t)\]
To ensure the same degree, it becomes:
\[y(t)=\dfrac{z^{2}-\frac{8}{3}z-1}{z^2+\frac{2}{3}z^1+\frac{1}{9}}\frac{3}{\frac{1}{2}}z^{-2}e(t)\]
Now, define the new White Noise as:
\[\eta(t)=\frac{3}{\frac{1}{2}}z^{-2}e(t)\rightarrow \eta(t)\sim WN\left(0,36\right)\]
Thus, we have:
\[y(t)=\dfrac{1-\frac{8}{3}z^{-1}-z^{-2}}{1+\frac{2}{3}z^{-1}+\frac{1}{9}z^{-2}}\eta(t) \qquad \eta(t)\sim WN\left(0,36\right)\]
The poles are at $z_{1,2}=-\frac{1}{3}$, and the zeros are at $z_{1,2}=-\frac{1}{3},3$. 
We have a zero that is not inside the unit circle.

Next, factorize the numerator and denominator:
\[y(t)=\dfrac{\left(1+\frac{1}{3}z^{-1}\right)\left(1-3z^{-1}\right)}{\left(1+\frac{1}{3}z^{-1}\right)\left(1+\frac{1}{3}z^{-1}\right)}\eta(t)=\dfrac{1-3z^{-1}}{1+\frac{1}{3}z^{-1}}\eta(t) \]
Use an all-pass filter to remove the zero at three:
\[y(t)=\dfrac{1-3z^{-1}}{1+\frac{1}{3}z^{-1}}\dfrac{1-\frac{1}{3}z^{-1}}{1+\frac{1}{3}z^{-1}}\eta(t)\]
Redefined the White Noise as:
\[\xi(t)=\dfrac{1-3z^{-1}}{1+\frac{1}{3}z^{-1}}\eta(t)\rightarrow \xi(t)\sim WN(0,324)\]

The canonical form is:
\[y(t)=\dfrac{1-\frac{1}{3}z^{-1}}{1+\frac{1}{3}z^{-1}}\xi(t)\]

Now, with the canonical representation, compute the one-step ahead predictor as:
\[\hat{y}(t|t-1)=\dfrac{C(z)-A(z)}{C(z)}y(t)=\dfrac{1+\frac{1}{3}z^{-1}-\left(1-\frac{1}{3}z^{-1}\right)}{1+\frac{1}{3}z^{-1}}y(t)=\dfrac{-\frac{2}{3}z^{-1}}{1-\frac{1}{3}z^{-1}}y(t)\]