\section{Exercise four}

Consider the process: 
\[y(t)=3+v(t)\]
Let's find the predictor $\hat{y}(t|t-k)$ for all $k$ when: 
\begin{enumerate}
    \item $v(t)\sim WN(0,1)$
    \item $v(t)=e(t)+\frac{1}{2}e(t-2)\quad e(t)\sim WN(0,1)$
\end{enumerate}

\subsection*{Solution}
\begin{enumerate}
    \item In this case, the process becomes:
        \[y(t)=3+v(t) \qquad v(t)\sim WN(0,1)\]
        The only predictable part at any time different from zero is the constant, so:
        \[\hat{y}(t|t-k)=3\]
    \item Here, the process becomes:
        \[y(t)=3+e(t)+\frac{1}{2}e(t-2)\quad e(t)\sim WN(0,1)\]
        The expected value of the process is three, so we consider the unbiased process:
        \[\tilde{y}(t)=y(t)-3\]
        Thus,
        \[\tilde{y}(t)=e(t)+\frac{1}{2}e(t-2)=\dfrac{1+\frac{1}{2}z^{-2}}{1}e(t)\]

        The process is in canonical form. 
        With long division, we get $F_1(z)=\frac{1}{2}z^{-2}$, $F_2(z)=\frac{1}{2}z^{-2}$, and $F_{3\rightarrow\infty}=0$. 

        For the one-step ahead predictor: 
        \[\hat{\tilde{y}}(t|t-1)=\dfrac{\frac{1}{2}z^{-2}}{1+\frac{1}{2}z^{-2}}\tilde{y}(t)=-\dfrac{1}{2}\tilde{y}(t-2|t-3)+\dfrac{1}{2}\tilde{y}(t-2)\]
        Thus, 
        \[\hat{y}(t|t-1)=-\dfrac{1}{2}y(t-2|t-3)+\dfrac{1}{2}y(t-2)+3\]

        For the two-step predictor: 
        \[\hat{y}(t|t-2)=-\dfrac{1}{2}y(t-2|t-4)+\dfrac{1}{2}y(t-2)+3\]

        For the general $k$: 
        \[\hat{y}(t|t-k)=3\]
\end{enumerate}