\section{Exercise five}

Consider the process: 
\[y(t)=\dfrac{1}{4}y(t-2)+\eta(t-2)+\dfrac{1}{3}\eta(t-3)\qquad \eta(t)\sim WN(0,1)\]
Let's compute the predictor $\hat{y}(t|t-2)$. 

\subsection*{Solution}
The transfer function of the expression is:
\[y(t)=\dfrac{z^{-1}+\frac{1}{3}z^{-3}}{1-\frac{1}{4}z^{-2}}\eta(t)=\dfrac{z^3+\frac{1}{3}z}{z^3-\frac{1}{4}z}\eta(t)\]

In canonical form it becomes: 
\[y(t)=\dfrac{1+\frac{1}{3}z^{-2}}{1-\frac{1}{4}z^{-2}}(t)\qquad e(t)\sim WN(0,1)\]
All the poles and zeros are inside the unit circle, so the transfer function is stable.

By performing the long division for two steps, we get $F_2(z)=\frac{7}{12}z^{-2}$ and $E(z)=1$. 
The predictor is: 
\[\hat{y}(t|t-2)=e(t)+\dfrac{\frac{7}{12}}{1-\frac{1}{4}z^{-2}}e(t-2)=\dfrac{\frac{7}{12}z^{-2}}{1-\frac{1}{4}z^{-2}}e(t)\]

In terms of data, it becomes:
\[\hat{y}(t|t-2)=\dfrac{\frac{7}{12}z^{-2}}{1-1\frac{1}{4}z^{-2}}\dfrac{1-\frac{1}{4}z^{-2}}{1+\frac{1}{3}z^{-2}}y(t)=\dfrac{\frac{7}{12}z^{-2}}{1+\frac{1}{3}z^{-2}}y(t)\]

In the time domain:
\[\hat{y}(t|t-2)=\frac{7}{12}y(t-2)-\frac{1}{3}z^{-2}\hat{y}(t-2|t-4)\]